Steel.Repr.Fun -> Repr.Fun
Repr.Fun is parametrized by a representation of the returned values and
associated quantifiers

experiment/Experiment.Repr.Fun.fst
@@ -1,47 +1,101 @@
 module Experiment.Repr.Fun
 
-(* TODO? (a : Type)  --->  (ts : ty_list) *)
+module U = Learn.Util
+
 
 noeq
-type prog_tree : (a : Type) -> Type =
-  | Tnew   : (a : Type) -> prog_tree a
-  | Tasrt  : (p : prop) -> prog_tree unit
-  | Tasum  : (p : prop) -> prog_tree unit
-  | Tret   : (a : Type) -> (x : a) -> prog_tree a
-  | Tbind  : (a : Type) -> (b : Type) ->
-             (f : prog_tree a) -> (g : a -> prog_tree b) ->
-             prog_tree b
-  | TbindP : (a : Type) -> (b : Type) ->
-             (wp : pure_wp a) -> (x : unit -> PURE a wp) -> (g : a -> prog_tree b) ->
-             prog_tree b
+type tys' = {
+  t : Type u#t;
+  v : t -> Type u#v;
+  unit : t;
+  emp  : v unit;
+  all  : (ty : t) -> (v ty -> Type0) -> Type0;
+  ex   : (ty : t) -> (v ty -> Type0) -> Type0;
+}
 
-let return (#a : Type) (x : a) : prog_tree a
+type tys = s : tys' {
+  (forall (x : s.v s.unit) . x == s.emp) /\
+  (forall (ty : s.t) (f : s.v ty -> Type0) . s.all ty f <==> (forall (x : s.v ty) . f x)) /\
+  (forall (ty : s.t) (f : s.v ty -> Type0) . s.ex  ty f <==> (exists (x : s.v ty) . f x))
+}
+
+let can_tys : tys u#(v+1) u#v = {
+  t = Type u#v;
+  v = (fun ty -> ty);
+  unit = U.unit';
+  emp  = U.Unit';
+  all  = (fun ty p -> forall (x : ty) . p x);
+  ex   = (fun ty p -> exists (x : ty) . p x)
+}
+
+noeq
+type prog_tree (s : tys u#t u#v) : s.t -> Type u#(max t v a + 1) =
+  | Tnew   : (a : s.t) -> prog_tree s a
+  | Tasrt  : (p : prop) -> prog_tree s s.unit
+  | Tasum  : (p : prop) -> prog_tree s s.unit
+  | Tspec  : (a : s.t) -> (pre : pure_pre) -> (post : pure_post (s.v a)) ->
+             prog_tree s a
+  | Tret   : (a : s.t) -> (x : s.v a) -> prog_tree s a
+  | Tbind  : (a : s.t) -> (b : s.t) ->
+             (f : prog_tree s a) -> (g : s.v a -> prog_tree s b) ->
+             prog_tree s b
+  (* [a] could be of type [s.t] *)
+  | TbindP : (a : Type u#a) -> (b : s.t) ->
+             (wp : pure_wp a) -> (x : unit -> PURE a wp) -> (g : a -> prog_tree s b) ->
+             prog_tree s b
+
+
+let return (#s : tys) (#a : s.t) ($x : s.v a) : prog_tree s a
   = Tret a x
 
-let bind (#a #b : Type) (f : prog_tree a) (g : a -> prog_tree b) : prog_tree b
+let bind (#s : tys) (#a #b : s.t) (f : prog_tree s a) (g : s.v a -> prog_tree s b) : prog_tree s b
   = Tbind a b f g
 
 
-let rec tree_req (#a : Type) (t : prog_tree a)
+let rec tree_req (#s : tys) (#a : s.t) (t : prog_tree s a)
   : Tot pure_pre (decreases t)
   = match t with
   | Tnew   _          -> True
   | Tasrt  p          -> p
   | Tasum  _          -> True
+  | Tspec  _ pre _    -> pre
   | Tret   _ _        -> True
-  | Tbind  a _ f g    -> tree_req f /\ (forall (x : a) . tree_ens f x ==> tree_req (g x))
-  | TbindP a _ wp _ g -> wp (fun x -> tree_req (g x)) /\ True
+  | Tbind  a b f g    -> tree_req f /\ s.all a (fun (x : s.v a) -> tree_ens f x ==> tree_req (g x))
+  | TbindP a _ wp _ g -> wp (fun x -> tree_req (g x))
 
-and tree_ens (#a : Type) (t : prog_tree a)
-  : Tot (pure_post a) (decreases t)
+and tree_ens (#s : tys) (#a : s.t) (t : prog_tree s a)
+  : Tot (pure_post (s.v a)) (decreases t)
   = match t with
   | Tnew   _          -> fun _  -> True
-  | Tasrt  p          -> fun () -> True (* p ?*)
-  | Tasum  p          -> fun () -> p
+  | Tasrt  p          -> fun _(*()*) -> True (* p ?*)
+  | Tasum  p          -> fun _(*()*) -> p
+  | Tspec  a _ post   -> post
   | Tret   _ x        -> fun r  -> r == x
-  | Tbind  a _ f g    -> fun y  -> exists (x : a) . tree_ens f x /\ tree_ens (g x) y
-  | TbindP a _ wp _ g -> fun y -> as_requires wp /\ (exists (x : a) . as_ensures wp x /\ tree_ens (g x) y)
+  | Tbind  a _ f g    -> fun y  -> s.ex a (fun (x : s.v a) -> tree_ens f x /\ tree_ens (g x) y)
+  | TbindP a _ wp _ g -> fun y -> (exists (x : a) . as_ensures wp x /\ tree_ens (g x) y)
 
+
+(*** Equivalence *)
+
+let equiv (#s : tys) (#a : s.t) (f g : prog_tree s a) : prop =
+  (tree_req f <==> tree_req g) /\
+  (tree_req f ==> (forall (x : s.v a) . tree_ens f x <==> tree_ens g x))
+
+
+let equiv_refl (#s : tys) (#a : s.t) (f : prog_tree s a)
+  : Lemma (equiv f f)
+  = ()
+
+let equiv_sym (#s : tys) (#a : s.t) (f g : prog_tree s a)
+  : Lemma (requires equiv f g) (ensures equiv g f)
+  = ()
+
+let equiv_trans (#s : tys) (#a : s.t) (f g h : prog_tree s a)
+  : Lemma (requires equiv f g /\ equiv g h) (ensures equiv f h)
+  = ()
+
+
+(*** Weakest-precondition *)
 
 module MP = FStar.Monotonic.Pure
 module T  = FStar.Tactics
@@ -49,35 +103,37 @@ module U  = Learn.Util
 open FStar.Classical.Sugar
 
 
-let rec tree_wp (#a : Type) (t : prog_tree a)
-  : Tot (pure_wp a) (decreases t)
+let rec tree_wp (#s : tys) (#a : s.t) (t : prog_tree s a)
+  : Tot (pure_wp (s.v a)) (decreases t)
   = match t with
-  | Tnew  a           -> MP.as_pure_wp (fun pt -> forall (x : a) . pt x)
-  | Tasrt p           -> MP.as_pure_wp (fun pt -> p /\ (p ==> pt ()))
-  | Tasum p           -> MP.as_pure_wp (fun pt -> p ==> pt ())
+  | Tnew  a           -> MP.as_pure_wp (fun pt -> s.all a (fun (x : s.v a) -> pt x))
+  | Tasrt p           -> MP.as_pure_wp (fun pt -> p /\ (p ==> pt s.emp))
+  | Tasum p           -> MP.as_pure_wp (fun pt -> p ==> pt s.emp)
+  | Tspec a pre post  -> MP.as_pure_wp (fun pt -> pre /\ s.all a (fun (x : s.v a) -> post x ==> pt x))
   | Tret  _ x         -> MP.as_pure_wp (fun pt -> pt x)
   | Tbind a _ f g     -> MP.elim_pure_wp_monotonicity_forall ();
-                        MP.as_pure_wp (fun pt -> tree_wp f (fun (x : a) -> tree_wp (g x) pt))
+                        MP.as_pure_wp (fun pt -> tree_wp f (fun (x : s.v a) -> tree_wp (g x) pt))
   | TbindP a _ wp _ g -> MP.elim_pure_wp_monotonicity_forall ();
                         MP.as_pure_wp (fun pt -> wp (fun (x : a) -> tree_wp (g x) pt))
 
-let rec tree_wp_sound (#a : Type) (t : prog_tree a) (post : pure_post a)
+let rec tree_wp_sound (#s : tys) (#a : s.t) (t : prog_tree s a) (post : pure_post (s.v a))
   : Lemma (requires tree_wp t post)
-          (ensures  tree_req t /\ (forall (x : a) . tree_ens t x ==> post x))
+          (ensures  tree_req t /\ (forall (x : s.v a) . tree_ens t x ==> post x))
+          (decreases t)
   = match t with
-  | Tnew _ | Tasrt _ | Tasum _ | Tret _ _ -> ()
+  | Tnew _ | Tasrt _ | Tasum _ | Tret _ _ | Tspec _ _ _ -> ()
   | Tbind a b f g ->
-      let post1 (x : a) = tree_wp (g x) post in
+      let post1 (x : s.v a) = tree_wp (g x) post in
       assert (tree_wp (Tbind a b f g) post == tree_wp f post1) by T.(trefl ());
       tree_wp_sound f post1;
-      introduce forall (x : a) . tree_wp (g x) post ==> (tree_req (g x) /\ (forall (y : b) . tree_ens (g x) y ==> post y))
+      introduce forall (x : s.v a) . tree_wp (g x) post ==> (tree_req (g x) /\ (forall (y : s.v b) . tree_ens (g x) y ==> post y))
         with introduce _ ==> _ with _ . tree_wp_sound (g x) post
   | TbindP a b wp xf g ->
       let post1 (x : a) = tree_wp (g x) post in
       let req1  (x : a) = tree_req (g x)     in
       assert (tree_wp (TbindP a b wp xf g) post == wp post1) by T.(trefl ());
       MP.elim_pure_wp_monotonicity wp;
-      introduce forall (x : a) . post1 x ==> (req1 x /\ (forall (y : b) . tree_ens (g x) y ==> post y))
+      introduce forall (x : a) . post1 x ==> (req1 x /\ (forall (y : s.v b) . tree_ens (g x) y ==> post y))
         with introduce _ ==> _ with _ . tree_wp_sound (g x) post;
-      assert (tree_req (TbindP a b wp xf g) == (wp req1 /\ True)) by T.(trefl ());
-      U.prop_equal (fun p -> p) (wp req1 /\ True) (tree_req (TbindP a b wp xf g))
+      assert (tree_req (TbindP a b wp xf g) == (wp req1)) by T.(trefl ());
+      U.prop_equal (fun p -> p) (wp req1) (tree_req (TbindP a b wp xf g))
